lifting typing spec

deps/poulet4/lib/P4cub/Semantics/Static/Typing.v
@@ -5,73 +5,66 @@ Require Import Coq.PArith.BinPos Coq.ZArith.BinInt Coq.NArith.BinNat
 From RecordUpdate Require Import RecordSet.
 Import String AllCubNotations Clmt.Notations RecordSetNotations.
 
-
 (** * Expression typing. *)
 
-Record expr_type_env : Set :=
-  mk_expr_type_env { type_vars:nat; types:list Expr.t }.
-
-Global Instance eta_expr_type_env : Settable _ :=
-  settable! mk_expr_type_env < type_vars ; types >.
-
-Reserved Notation "Γ '⊢ₑ' e ∈ τ" (at level 80, no associativity).
+Reserved Notation "'`⟨' Δ , Γ ⟩ ⊢ e ∈ τ" (at level 80, no associativity).
 
 Local Open Scope ty_scope.
 Local Open Scope expr_scope.
 
-Inductive type_expr (Γ : expr_type_env)
+Inductive type_expr (Δ : nat) (Γ : list Expr.t)
   : Expr.e -> Expr.t -> Prop :=
 | type_bool (b : bool) :
-  Γ ⊢ₑ b ∈ Expr.TBool
+  `⟨ Δ, Γ ⟩ ⊢ b ∈ Expr.TBool
 | type_bit w n :
   BitArith.bound w n ->
-  Γ ⊢ₑ w `W n ∈ Expr.TBit w
+  `⟨ Δ, Γ ⟩ ⊢ w `W n ∈ Expr.TBit w
 | type_int w n :
   IntArith.bound w n ->
-  Γ ⊢ₑ w `S n ∈ Expr.TInt w
+  `⟨ Δ, Γ ⟩ ⊢ w `S n ∈ Expr.TInt w
 | type_var τ og x :
-  nth_error (types Γ) x = Some τ ->
-  t_ok (type_vars Γ) τ ->
-  Γ ⊢ₑ Expr.Var τ og x ∈ τ
+  nth_error Γ x = Some τ ->
+  t_ok Δ τ ->
+  `⟨ Δ, Γ ⟩ ⊢ Expr.Var τ og x ∈ τ
 | type_slice hi lo e w τ :
   (Npos lo <= Npos hi < w)%N ->
   numeric_width w τ ->
-  Γ ⊢ₑ e ∈ τ ->
-  Γ ⊢ₑ Expr.Slice hi lo e ∈ Expr.TBit (Npos hi - Npos lo + 1)%N
+  `⟨ Δ, Γ ⟩ ⊢ e ∈ τ ->
+  `⟨ Δ, Γ ⟩ ⊢ Expr.Slice hi lo e ∈ Expr.TBit (Npos hi - Npos lo + 1)%N
 | type_cast τ τ' e :
   proper_cast τ' τ ->
-  t_ok (type_vars Γ) τ ->
-  Γ ⊢ₑ e ∈ τ' ->
-  Γ ⊢ₑ Expr.Cast τ e ∈ τ
+  t_ok Δ τ ->
+  `⟨ Δ, Γ ⟩ ⊢ e ∈ τ' ->
+  `⟨ Δ, Γ ⟩ ⊢ Expr.Cast τ e ∈ τ
 | type_uop op τ τ' e :
   uop_type op τ τ' ->
-  t_ok (type_vars Γ) τ' ->
-  Γ ⊢ₑ e ∈ τ ->
-  Γ ⊢ₑ Expr.Uop τ' op e ∈ τ'
+  t_ok Δ τ' ->
+  `⟨ Δ, Γ ⟩ ⊢ e ∈ τ ->
+  `⟨ Δ, Γ ⟩ ⊢ Expr.Uop τ' op e ∈ τ'
 | type_bop op τ₁ τ₂ τ e₁ e₂ :
   bop_type op τ₁ τ₂ τ ->
-  t_ok (type_vars Γ) τ ->
-  Γ ⊢ₑ e₁ ∈ τ₁ ->
-  Γ ⊢ₑ e₂ ∈ τ₂ ->
-  Γ ⊢ₑ Expr.Bop τ op e₁ e₂ ∈ τ
+  t_ok Δ τ ->
+  `⟨ Δ, Γ ⟩ ⊢ e₁ ∈ τ₁ ->
+  `⟨ Δ, Γ ⟩ ⊢ e₂ ∈ τ₂ ->
+  `⟨ Δ, Γ ⟩ ⊢ Expr.Bop τ op e₁ e₂ ∈ τ
 | type_index e₁ e₂ w τ :
-  t_ok (type_vars Γ) τ ->
-  Γ ⊢ₑ e₁ ∈ Expr.TArray (Z.to_N (BitArith.upper_bound w)) τ ->
-  Γ ⊢ₑ e₂ ∈ Expr.TBit w ->
-  Γ ⊢ₑ Expr.Index τ e₁ e₂ ∈ τ
+  t_ok Δ τ ->
+  `⟨ Δ, Γ ⟩ ⊢ e₁ ∈ Expr.TArray (Z.to_N (BitArith.upper_bound w)) τ ->
+  `⟨ Δ, Γ ⟩ ⊢ e₂ ∈ Expr.TBit w ->
+  `⟨ Δ, Γ ⟩ ⊢ Expr.Index τ e₁ e₂ ∈ τ
 | type_member τ x e τs b :
   nth_error τs x = Some τ ->
-  t_ok (type_vars Γ) τ ->
-  Γ ⊢ₑ e ∈ Expr.TStruct b τs ->
-  Γ ⊢ₑ Expr.Member τ x e ∈ τ
+  t_ok Δ τ ->
+  `⟨ Δ, Γ ⟩ ⊢ e ∈ Expr.TStruct b τs ->
+  `⟨ Δ, Γ ⟩ ⊢ Expr.Member τ x e ∈ τ
 | type_lists ls es τ τs :
-  t_ok_lists (type_vars Γ) ls ->
+  t_ok_lists Δ ls ->
   type_lists_ok ls τ τs ->
-  Forall2 (type_expr Γ) es τs ->
-  Γ ⊢ₑ Expr.Lists ls es ∈ τ
+  Forall2 (type_expr Δ Γ) es τs ->
+  `⟨ Δ, Γ ⟩ ⊢ Expr.Lists ls es ∈ τ
 | type_error err :
-  Γ ⊢ₑ Expr.Error err ∈ Expr.TError
-where "Γ '⊢ₑ' e ∈ τ" := (type_expr Γ e τ) : type_scope.
+  `⟨ Δ, Γ ⟩ ⊢ Expr.Error err ∈ Expr.TError
+where "'`⟨' Δ , Γ ⟩ ⊢ e ∈ τ" := (type_expr Δ Γ e τ) : type_scope.
 
 Local Close Scope expr_scope.
 Local Open Scope pat_scope.
@@ -98,122 +91,107 @@ Local Close Scope pat_scope.
 
 (** Parser-expression typing. *)
 Variant type_prsrexpr 
-        (total_states : nat) (Γ : expr_type_env)
+        (total_states : nat) (Δ : nat) (Γ : list Expr.t)
   : Parser.pt -> Prop :=
   | type_goto (st : Parser.state_label) :
     valid_state total_states st ->
-    type_prsrexpr total_states Γ (Parser.Direct st)
+    type_prsrexpr total_states Δ Γ (Parser.Direct st)
   | type_select e default cases τ :
     valid_state total_states default ->
-    Γ ⊢ₑ e ∈ τ ->
+    `⟨ Δ, Γ ⟩ ⊢ e ∈ τ ->
     Forall
       (fun '(p,st) => type_pat p τ /\ valid_state total_states st)
       cases ->
-    type_prsrexpr total_states Γ (Parser.Select e default cases).
+    type_prsrexpr total_states Δ Γ (Parser.Select e default cases).
 
 (** * Statement typing. *)
-
-Record stmt_type_env : Set :=
-  mk_stmt_type_env
-    { sfuncts : fenv
-    ; cntx   : ctx
-    ; expr_env :> expr_type_env }.
-
-Global Instance eta_stmt_type_env : Settable _ :=
-  settable! mk_stmt_type_env < sfuncts ; cntx ; expr_env >.
-
-Inductive type_fun_kind (Γ : stmt_type_env)
+Inductive type_fun_kind
+  (Δ : nat) (Γ : list Expr.t) (fs : fenv) (c : ctx)
     : Stmt.fun_kind -> list Expr.t -> Expr.params -> Prop :=
 | type_call_funct f τs oe params ot :
-  sfuncts Γ f = Some (List.length τs, {|paramargs:=params; rtrns:=ot|}) ->
+  fs f = Some (List.length τs, {|paramargs:=params; rtrns:=ot|}) ->
   predop lvalue_ok oe ->
-  relop (type_expr Γ) oe (option_map (tsub_t (gen_tsub τs)) ot) ->
-  type_fun_kind Γ (Stmt.Funct f τs oe) τs params
+  relop (type_expr Δ Γ) oe (option_map (tsub_t (gen_tsub τs)) ot) ->
+  type_fun_kind Δ Γ fs c (Stmt.Funct f τs oe) τs params
 | type_call_action a cargs aa cparams params :
-  action_call_ok aa (cntx Γ) ->
+  action_call_ok aa c ->
   aa a = Some (cparams,params) ->
-  Forall2 (type_expr Γ) cargs cparams ->
-  type_fun_kind Γ (Stmt.Action a cargs) [] params
+  Forall2 (type_expr Δ Γ) cargs cparams ->
+  type_fun_kind Δ Γ fs c (Stmt.Action a cargs) [] params
 | type_call_method ei m τs oe params ot extern_insts methods :
-  extern_call_ok extern_insts (cntx Γ) ->
+  extern_call_ok extern_insts c ->
   extern_insts ei = Some (inl methods) ->
   Field.get m methods = Some (List.length τs, {|paramargs:=params; rtrns:=ot|}) ->
   predop lvalue_ok oe ->
-  relop (type_expr Γ) oe (option_map (tsub_t (gen_tsub τs)) ot) ->
-  type_fun_kind Γ (Stmt.Method ei m τs oe) τs params.
+  relop (type_expr Δ Γ) oe (option_map (tsub_t (gen_tsub τs)) ot) ->
+  type_fun_kind Δ Γ fs c (Stmt.Method ei m τs oe) τs params.
 
-Reserved Notation "Γ '⊢ₛ' s ⊣ sig" (at level 80, no associativity).
+Reserved Notation "'`⧼' Δ , Γ , f , c ⧽ ⊢ s ⊣ sig" (at level 80, no associativity).
 
 Local Open Scope stmt_scope.
 
-Inductive type_stmt
-  : stmt_type_env -> Stmt.s -> signal -> Prop :=
-| type_skip Γ :
-  Γ ⊢ₛ Stmt.Skip ⊣ Cont
-| type_return Γ eo :
-  match cntx Γ, eo with
-  | CFunction (Some τ), Some e => Γ ⊢ₑ e ∈ τ
+Inductive type_stmt (Δ : nat) (Γ : list Expr.t) (fs : fenv)
+  : ctx -> Stmt.s -> signal -> Prop :=
+| type_skip c :
+  `⧼ Δ, Γ, fs, c ⧽ ⊢ Stmt.Skip ⊣ Cont
+| type_return c eo :
+  match c, eo with
+  | CFunction (Some τ), Some e => `⟨ Δ, Γ ⟩ ⊢ e ∈ τ
   | c, None => return_void_ok c
   | _, _ => False
   end ->
-  Γ ⊢ₛ Stmt.Return eo ⊣ Return
-| type_exit Γ :
-  exit_ctx_ok (cntx Γ) ->
-  Γ ⊢ₛ Stmt.Exit ⊣ Exit
-| type_transition (Γ : stmt_type_env) total_states e :
-  transition_ok total_states (cntx Γ) ->
-  type_prsrexpr total_states Γ e ->
-  Γ ⊢ₛ Stmt.Transition e ⊣ Trans
-| type_assign (Γ : stmt_type_env) τ e₁ e₂ :
+  `⧼ Δ, Γ, fs, c ⧽ ⊢ Stmt.Return eo ⊣ Return
+| type_exit c :
+  exit_ctx_ok c ->
+  `⧼ Δ, Γ, fs, c ⧽ ⊢ Stmt.Exit ⊣ Exit
+| type_transition total_states i e :
+  type_prsrexpr total_states Δ Γ e ->
+  `⧼ Δ, Γ, fs, CParserState total_states i ⧽ ⊢ Stmt.Transition e ⊣ Trans
+| type_assign c τ e₁ e₂ :
   lvalue_ok e₁ ->
-  Γ ⊢ₑ e₁ ∈ τ ->
-  Γ ⊢ₑ e₂ ∈ τ ->
-  Γ ⊢ₛ e₁ `:= e₂ ⊣ Cont
-| type_fun_call Γ params τs args fk :
-  type_fun_kind Γ fk τs params ->
-  Forall (t_ok (type_vars Γ)) τs ->
+  `⟨ Δ, Γ ⟩ ⊢ e₁ ∈ τ ->
+  `⟨ Δ, Γ ⟩ ⊢ e₂ ∈ τ ->
+  `⧼ Δ, Γ, fs, c ⧽ ⊢ e₁ `:= e₂ ⊣ Cont
+| type_fun_call c params τs args fk :
+  type_fun_kind Δ Γ fs c fk τs params ->
+  Forall (t_ok Δ) τs ->
   Forall2
     (rel_paramarg
-       (type_expr Γ)
-       (fun e τ => Γ ⊢ₑ e ∈ τ /\ lvalue_ok e))
+       (type_expr Δ Γ)
+       (fun e τ => `⟨ Δ, Γ ⟩ ⊢ e ∈ τ /\ lvalue_ok e))
     args (map (tsub_param (gen_tsub τs)) (map snd params)) ->
-  Γ ⊢ₛ Stmt.Call fk args ⊣ Cont
+  `⧼ Δ, Γ, fs, c ⧽ ⊢ Stmt.Call fk args ⊣ Cont
 | type_apply
-    Γ extern_args args x extern_params params sig insts :
-  apply_instance_ok insts sig (cntx Γ) ->
+    c extern_args args x extern_params params sig insts :
+  apply_instance_ok insts sig c ->
   insts x = Some (inr (sig,extern_params,params)) ->
   Forall2
     (rel_paramarg
-       (type_expr Γ)
-       (fun e τ => Γ ⊢ₑ e ∈ τ /\ lvalue_ok e))
+       (type_expr Δ Γ)
+       (fun e τ => `⟨ Δ, Γ ⟩ ⊢ e ∈ τ /\ lvalue_ok e))
     args (map snd params) ->
-  Γ ⊢ₛ Stmt.Apply x extern_args args ⊣ Cont
-| type_invoke
-    Γ tbl tbls :
-  table_invoke_ok tbls (cntx Γ) ->
+  `⧼ Δ, Γ, fs, c ⧽ ⊢ Stmt.Apply x extern_args args ⊣ Cont
+| type_invoke tbl tbls aa i :
   In tbl tbls ->
-  Γ ⊢ₛ Stmt.Invoke tbl ⊣ Cont
-| type_vardecl (Γ : stmt_type_env) og τ te s sig :
+  `⧼ Δ, Γ, fs, CApplyBlock tbls aa i ⧽ ⊢ Stmt.Invoke tbl ⊣ Cont
+| type_vardecl c og τ te s sig :
     match te with
-    | inr e => Γ ⊢ₑ e ∈ τ
-    | inl τ' => τ' = τ /\ t_ok (type_vars Γ) τ'
+    | inr e => `⟨ Δ, Γ ⟩ ⊢ e ∈ τ
+    | inl τ' => τ' = τ /\ t_ok Δ τ'
     end ->
-    (Γ <| expr_env :=
-       Γ.(expr_env)
-           <| types :=
-         τ :: Γ.(types) |> |>) ⊢ₛ s ⊣ sig ->
-    Γ ⊢ₛ Stmt.Var og te s ⊣ sig
-| type_seq Γ s₁ s₂ sig₁ sig₂ :
-  Γ ⊢ₛ s₁ ⊣ sig₁ ->
-  Γ ⊢ₛ s₂ ⊣ sig₂ ->
-  Γ ⊢ₛ s₁ `; s₂ ⊣ sig₂
-| type_cond (Γ : stmt_type_env) e s₁ s₂ sig₁ sig₂ sig :
+    `⧼ Δ, τ :: Γ, fs, c ⧽ ⊢ s ⊣ sig ->
+    `⧼ Δ, Γ, fs, c ⧽ ⊢ Stmt.Var og te s ⊣ sig
+| type_seq c s₁ s₂ sig₁ sig₂ :
+  `⧼ Δ, Γ, fs, c ⧽ ⊢ s₁ ⊣ sig₁ ->
+  `⧼ Δ, Γ, fs, c ⧽ ⊢ s₂ ⊣ sig₂ ->
+  `⧼ Δ, Γ, fs, c ⧽ ⊢ s₁ `; s₂ ⊣ sig₂
+| type_cond c e s₁ s₂ sig₁ sig₂ sig :
   lub sig₁ sig₂ = Some sig ->
-  Γ ⊢ₑ e ∈ Expr.TBool ->
-  Γ ⊢ₛ s₁ ⊣ sig₁ ->
-  Γ ⊢ₛ s₂ ⊣ sig₂ ->
-  Γ ⊢ₛ If e Then s₁ Else s₂ ⊣ sig
-where "Γ '⊢ₛ' s ⊣ sig" := (type_stmt Γ s sig).
+  `⟨ Δ, Γ ⟩ ⊢ e ∈ Expr.TBool ->
+  `⧼ Δ, Γ, fs, c ⧽ ⊢ s₁ ⊣ sig₁ ->
+  `⧼ Δ, Γ, fs, c ⧽ ⊢ s₂ ⊣ sig₂ ->
+  `⧼ Δ, Γ, fs, c ⧽ ⊢ If e Then s₁ Else s₂ ⊣ sig
+where "'`⧼' Δ , Γ , fs , c ⧽ '⊢' s ⊣ sig" := (type_stmt Δ Γ fs c s sig).
 
 Local Close Scope stmt_scope.
 
@@ -222,7 +200,8 @@ Local Close Scope stmt_scope.
 (** Control-declaration typing context. *)
 Record ctrl_type_env : Set :=
   mk_ctrl_type_env
-    { cexpr_env : expr_type_env
+    { ctype_vars : nat
+    ; ctypes : list Expr.t
     ; cfuncts : fenv (** available functions. *)
     ; cinsts : ienv  (** available control instances. *)
     ; actns : aenv   (** available action signatures. *)
@@ -230,7 +209,7 @@ Record ctrl_type_env : Set :=
 
 Global Instance eta_ctrl_type_env : Settable _ :=
   settable! mk_ctrl_type_env
-  < cexpr_env ; cfuncts ; cinsts ; actns ; tbls >.
+  < ctype_vars ; ctypes ; cfuncts ; cinsts ; actns ; tbls >.
 
 Reserved Notation "Γ '⊢ᵪ' d '⊣' result"
          (at level 80, no associativity).
@@ -247,24 +226,20 @@ Variant type_ctrldecl (Γ : ctrl_type_env)
   : Control.d -> ctrldecl_type -> Prop :=
   | type_ctrl_var x te τ :
     match te with
-    | inr e => cexpr_env Γ ⊢ₑ e ∈ τ
-    | inl τ' => τ' = τ /\ t_ok (type_vars $ cexpr_env Γ) τ'
+    | inr e => `⟨ ctype_vars Γ, ctypes Γ ⟩ ⊢ e ∈ τ
+    | inl τ' => τ' = τ /\ t_ok (ctype_vars Γ) τ'
     end ->
     Γ ⊢ᵪ Control.Var x te ⊣ ctrl_var_type τ
   | type_action action_name cparams dparams body sig :
-    {| sfuncts := cfuncts Γ
-    ; cntx     := CAction (actns Γ) (cinsts Γ)
-    ; expr_env :=
-        {| type_vars := type_vars (cexpr_env Γ)
-        ; types := map snd cparams ++ bind_all dparams (types (cexpr_env Γ)) |}
-    |} ⊢ₛ body ⊣ sig ->
+    `⧼ ctype_vars Γ, map snd cparams ++ bind_all dparams (ctypes Γ),
+        cfuncts Γ, CAction (actns Γ) (cinsts Γ) ⧽ ⊢ body ⊣ sig ->
     Γ ⊢ᵪ Control.Action action_name cparams dparams body
       ⊣ ctrl_act_type action_name (map snd cparams) dparams
   | type_table table_name key actions :
     (** Keys type. *)
     Forall
       (fun '(e,_) => exists τ,
-           cexpr_env Γ ⊢ₑ e ∈ τ) key ->
+           `⟨ ctype_vars Γ, ctypes Γ ⟩ ⊢ e ∈ τ) key ->
     (** Actions type *)
     Forall
       (fun '(a,data_args) =>
@@ -272,8 +247,8 @@ Variant type_ctrldecl (Γ : ctrl_type_env)
            actns Γ a = Some (ctrl_params, data_params)
            /\ Forall2
                (rel_paramarg
-                  (type_expr $ cexpr_env Γ)
-                  (fun e τ => cexpr_env Γ ⊢ₑ e ∈ τ /\ lvalue_ok e))
+                  (type_expr (ctype_vars Γ) $ ctypes Γ)
+                  (fun e τ => `⟨ ctype_vars Γ, ctypes Γ ⟩ ⊢ e ∈ τ /\ lvalue_ok e))
                data_args (List.map snd data_params))
       actions ->
     Γ ⊢ᵪ Control.Table
@@ -311,14 +286,15 @@ Definition type_ctrl
          Γ ⊢ᵪ d ⊣ result /\
            match result with
            | ctrl_var_type τ =>
-               Γ' = Γ <| cexpr_env := Γ.(cexpr_env) <| types := τ :: Γ.(cexpr_env).(types) |> |>
+               Γ' = Γ <| ctypes := τ :: Γ.(ctypes) |>
            | ctrl_act_type an cps dps =>
                Γ' = Γ <| actns := an ↦ (cps, dps) ,, actns Γ |>
            | ctrl_tbl_type tn =>
                Γ' = Γ <| tbls := tn :: tbls Γ |>
            end)
     ctrl
-    {| cexpr_env := {|type_vars:=0;types:=bind_all params Γ|}
+    {| ctype_vars := 0
+    ; ctypes := bind_all params Γ
     ; cfuncts := fs
     ; cinsts := cis
     ; actns := ∅ ; tbls := [] |}.
@@ -344,7 +320,7 @@ Inductive type_topdecl (Γ : top_type_env)
        | _ => False
        end) cargs cparams ->
   Forall2
-    (type_expr {| type_vars:=0; types:=[] |})
+    (type_expr 0 [])
     expr_cargs expr_cparams ->
   Γ ⊢ₜTopDecl.Instantiate
     control_decl_name instance_name [] cargs expr_cargs
@@ -370,7 +346,7 @@ Inductive type_topdecl (Γ : top_type_env)
        | _ => False
        end) cargs cparams ->
   Forall2
-    (type_expr {| type_vars:=0; types:=[] |})
+    (type_expr 0 [])
     expr_cargs expr_cparams ->
   Γ ⊢ₜTopDecl.Instantiate
     parser_decl_name instance_name [] cargs expr_cargs
@@ -398,7 +374,7 @@ Inductive type_topdecl (Γ : top_type_env)
        | _ => False
        end) cargs cparams ->
   Forall2
-    (type_expr {| type_vars:=0; types:=[] |})
+    (type_expr 0 [])
     expr_cargs expr_cparams ->
   Γ ⊢ₜTopDecl.Instantiate
     package_decl_name instance_name [] cargs expr_cargs
@@ -422,7 +398,7 @@ Inductive type_topdecl (Γ : top_type_env)
        end)
     cargs (map (tsub_cparam (gen_tsub τs)) cparams) ->
   Forall2
-    (type_expr {| type_vars:=0; types:=[] |})
+    (type_expr 0 [])
     expr_cargs (map (tsub_t (gen_tsub τs)) expr_cparams) ->
   Γ ⊢ₜ TopDecl.Instantiate extern_decl_name extern_name τs cargs expr_cargs
     ⊣ Γ <| insts_env := (* TODO: sub [τs] into methods *)
@@ -437,10 +413,9 @@ Inductive type_topdecl (Γ : top_type_env)
   insts = cbind_all (insts_env Γ) cparams ->
   type_ctrl
     params expr_cparams (tfuncts Γ) insts control_decls Γ' ->
-  {| expr_env := {|type_vars:=0;types:=bind_all params expr_cparams |}
-  ; sfuncts := tfuncts Γ
-  ; cntx := CApplyBlock (tbls Γ') (actns Γ') insts |}
-    ⊢ₛ apply_blk ⊣ sig ->
+  `⧼ 0, bind_all params expr_cparams,
+      tfuncts Γ, CApplyBlock (tbls Γ') (actns Γ') insts ⧽
+    ⊢ apply_blk ⊣ sig ->
   Γ ⊢ₜ
     TopDecl.Control
     control_name cparams expr_cparams extern_params
@@ -458,10 +433,8 @@ Inductive type_topdecl (Γ : top_type_env)
   insts = cbind_all (insts_env Γ) cparams ->
   Forall
     (fun state =>
-       {| sfuncts := tfuncts Γ
-       ;  cntx := CParserState (List.length states) insts
-       ;  expr_env := {|type_vars:=0;types:=bind_all params expr_cparams|}
-       |} ⊢ₛ state ⊣ Trans)
+       `⧼ 0, bind_all params expr_cparams, tfuncts Γ,
+           CParserState (List.length states) insts ⧽ ⊢ state ⊣ Trans)
     (start_state :: states) ->
   Γ ⊢ₜ TopDecl.Parser
     parser_decl_name cparams expr_cparams extern_params params
@@ -482,12 +455,8 @@ Inductive type_topdecl (Γ : top_type_env)
                 expr_cparams extern_name ,, cnstrs Γ |>
 | type_function function_name type_params arrow body sig :
   good_signal arrow sig ->
-  {| sfuncts := tfuncts Γ
-  ; cntx := CFunction (rtrns arrow)
-  ; expr_env :=
-    {| type_vars := type_params
-    ; types := bind_all (paramargs arrow) [] |}
-  |} ⊢ₛ body ⊣ sig ->
+  `⧼ type_params, bind_all (paramargs arrow) [], tfuncts Γ,
+      CFunction (rtrns arrow) ⧽ ⊢ body ⊣ sig ->
   Γ ⊢ₜ TopDecl.Funct
     function_name type_params arrow body
     ⊣ Γ <| tfuncts := function_name ↦ (type_params,arrow) ,, tfuncts Γ |>
