deps/poulet4/lib/P4cub/Transformations/Lifting/TypingSpec.v
@@ -4,7 +4,8 @@ Require Export Coq.micromega.Lia
 From Poulet4.P4cub Require Export Semantics.Static.Static
      Semantics.Static.Auxiliary
      Transformations.Lifting.Statementize.
-Import AllCubNotations.
+From RecordUpdate Require Import RecordSet.
+Import AllCubNotations RecordSetNotations.
 
 (** Typing specification for lifting in [Statementize.v] *)
 
@@ -13,7 +14,7 @@ Inductive type_decl_list (Δ : nat) (Γ : list Expr.t)
 | type_decl_nil :
   type_decl_list Δ Γ [] []
 | type_decl_cons h hτ t tτ :
-  {|type_vars:=Δ;types:=tτ ++ Γ|} ⊢ₑ h ∈ hτ ->
+  `⟨ Δ, tτ ++ Γ ⟩ ⊢ h ∈ hτ ->
   type_decl_list Δ Γ t tτ ->
   type_decl_list Δ Γ (h :: t) (hτ :: tτ).
 
@@ -43,12 +44,12 @@ Qed.
 Local Hint Resolve type_decl_list_append : core.
 Local Hint Constructors type_expr : core.
 
-Lemma shift_type : forall τs Γ e τ,
-    Γ ⊢ₑ e ∈ τ ->
-    {|type_vars:=type_vars Γ;types:=τs ++ types Γ|}
-      ⊢ₑ Shift.rename_e (Nat.add (length τs)) e ∈ τ.
+Lemma shift_type : forall τs Δ Γ e τ,
+    `⟨ Δ, Γ ⟩ ⊢ e ∈ τ ->
+    `⟨ Δ, τs ++ Γ ⟩
+      ⊢ Shift.rename_e (Nat.add (length τs)) e ∈ τ.
 Proof.
-  intros ts Γ e t het.
+  intros ts Δ Γ e t het.
   induction het using custom_type_expr_ind; unravel in *; eauto.
   - constructor; auto; unravel.
     rewrite nth_error_app3; assumption.
@@ -58,16 +59,6 @@ Proof.
 Qed.
 
 Local Hint Resolve shift_type : core.
-
-Lemma shift_type' : forall Δ τs Γ e τ,
-    {|type_vars:=Δ;types:=Γ|} ⊢ₑ e ∈ τ ->
-    {|type_vars:=Δ;types:=τs ++ Γ|}
-      ⊢ₑ Shift.rename_e (Nat.add (length τs)) e ∈ τ.
-Proof.
-  intros Δ ts Γ e t; apply shift_type.
-Qed.
-
-Local Hint Resolve shift_type' : core.
 Local Hint Constructors relop : core.
 Local Hint Constructors t_ok : core.
 Local Hint Resolve type_array : core.
@@ -76,16 +67,14 @@ Local Hint Resolve type_header : core.
 Local Hint Constructors type_lists_ok : core.
 Local Hint Constructors t_ok_lists : core.
 
-Theorem lift_e_type_expr : forall Γ e τ,
-    Forall (t_ok (type_vars Γ)) (types Γ) ->
-    Γ ⊢ₑ e ∈ τ -> forall us l e',
+Theorem lift_e_type_expr : forall Δ Γ e τ,
+    Forall (t_ok Δ) Γ ->
+    `⟨ Δ, Γ ⟩ ⊢ e ∈ τ -> forall us l e',
       lift_e (length us) e = (l, e') -> exists τs,
-        type_decl_list (type_vars Γ) (us ++ types Γ) l τs
-        /\ {| type_vars := type_vars Γ
-          ;  types     := τs ++ us ++ types Γ
-          |} ⊢ₑ e' ∈ τ.
+          type_decl_list Δ (us ++ Γ) l τs
+          /\ `⟨ Δ, τs ++ us ++ Γ ⟩ ⊢ e' ∈ τ.
 Proof.
-  intros Γ e t hΓ het;
+  intros Δ Γ e t hΓ het;
     induction het using custom_type_expr_ind;
     intros us l e' h; unravel in *.
   - inv h; eauto.
@@ -133,12 +122,10 @@ Proof.
       (lift_list lift_e Shift.rename_e (length us) es)
       as [les es'] eqn:eqles; inv h.
     assert (bruh : exists τs',
-               type_decl_list (type_vars Γ) (us ++ types Γ) les τs'
+               type_decl_list Δ (us ++ Γ) les τs'
                /\ Forall2
-                   (type_expr
-               {| type_vars:=type_vars Γ
-               ;  types := (τs' ++ us ++ types Γ) |})
-                   es' τs).
+                   (type_expr Δ (τs' ++ us ++ Γ))
+                      es' τs).
     { clear dependent ls.
       generalize dependent es';
         generalize dependent les;
@@ -162,13 +149,13 @@ Proof.
         constructor; rewrite <- app_assoc; eauto. }
     destruct bruh as (τs' & htτs' & ih).
     eexists; split; eauto; unravel.
-    assert (hok: t_ok (type_vars Γ) (Expr.TStruct false τs))
+    assert (hok: t_ok Δ (Expr.TStruct false τs))
       by eauto using type_expr_t_ok; inv hok.
     assert (bruh : map t_of_e es = τs).
     { rewrite Forall2_forall in H1.
       pose proof conj
            (proj1 H1)
-           (fun e τ hin => t_of_e_correct Γ e τ (proj2 H1 e τ hin)) as duh.
+           (fun e τ hin => t_of_e_correct Δ Γ e τ (proj2 H1 e τ hin)) as duh.
       rewrite <- Forall2_forall in duh; clear H1.
       rewrite ForallMap.Forall2_map_l,Forall2_eq in duh; assumption. }
     rewrite bruh.
@@ -179,18 +166,16 @@ Proof.
   - inv h; eauto.
 Qed.
 
-Lemma lift_e_list_type_expr : forall Γ es τs,
-    Forall (t_ok (type_vars Γ)) (types Γ) ->
-    Forall2 (type_expr Γ) es τs -> forall us les es',
+Lemma lift_e_list_type_expr : forall Δ Γ es τs,
+    Forall (t_ok Δ) Γ ->
+    Forall2 (type_expr Δ Γ) es τs -> forall us les es',
       lift_e_list (length us) es = (les, es') -> exists τs',
-        type_decl_list (type_vars Γ) (us ++ types Γ) les τs'
+        type_decl_list Δ (us ++ Γ) les τs'
         /\ Forall2
-            (type_expr
-               {| type_vars:=type_vars Γ
-               ;  types := (τs' ++ us ++ types Γ) |})
+            (type_expr Δ (τs' ++ us ++ Γ))
             es' τs.
 Proof.
-  intros G es ts hG hets;
+  intros D G es ts hG hets;
     induction hets as [| e t es ts het hests ih];
     intros us les es' h; unravel in *.
   - inv h; eauto.
@@ -208,3 +193,169 @@ Proof.
     rewrite hlesτs.
     constructor; rewrite <- app_assoc; eauto.
 Qed.
+
+Local Hint Constructors type_prsrexpr : core.
+
+Theorem lift_trans_type_expr : forall total_states Δ Γ p,
+    Forall (t_ok Δ) Γ ->
+    type_prsrexpr total_states Δ Γ p -> forall us l p',
+        lift_trans (length us) p = (l, p') -> exists τs,
+          type_decl_list Δ (us ++ Γ) l τs
+          /\ type_prsrexpr total_states Δ (τs ++ us ++ Γ) p'.
+Proof.
+  intros n D G p hok ht us l p' hlift.
+  inv ht; cbn in hlift.
+  - inv hlift. exists []; cbn; split; eauto.
+  - destruct (lift_e (length us) e) as [le e'] eqn:hlifte.
+    inv hlift.
+    pose proof lift_e_type_expr
+      _ _ _ _ hok H0 _ _ _ hlifte as (ts' & hts' & Hts').
+    exists ts'. split; eauto.
+Qed.
+
+Local Hint Constructors lvalue_ok : core.
+
+Lemma lvalue_rename_e : forall ρ e,
+    lvalue_ok e -> lvalue_ok (Shift.rename_e ρ e).
+Proof.
+  intros r e he; induction he; unravel; eauto.
+Qed.
+
+Local Hint Resolve lvalue_rename_e : core.
+
+Lemma lvalue_lift_e : forall e,
+    lvalue_ok e -> forall e' up l,
+      lift_e up e = (l, e') ->
+      lvalue_ok e'.
+Proof.
+  intros e he; induction he;
+    intros e' up le hlift; cbn in *.
+  - inv hlift; auto.
+  - destruct (lift_e up e) as [l' e''] eqn:he''.
+    inv hlift; auto.
+  - destruct (lift_e up e₁) as [l1 e1] eqn:he1.
+    destruct (lift_e (length l1 + up) e₂) as [l2 e2] eqn:he2.
+    inv hlift; unravel. eauto.
+  - destruct (lift_e up e) as [l' e''] eqn:he''.
+    inv hlift; eauto.
+Qed.
+
+Local Hint Resolve lvalue_lift_e : core.
+Local Hint Constructors type_fun_kind : core.
+Local Hint Constructors predop : core.
+
+Lemma type_fun_kind_lift : forall Δ Γ fs c fk τs params,
+    Forall (t_ok Δ) Γ ->
+    type_fun_kind Δ Γ fs c fk τs params -> forall us l fk',
+        lift_fun_kind (length us) fk = (l, fk') -> exists τs',
+          type_decl_list Δ (us ++ Γ) l τs'
+          /\ type_fun_kind Δ (τs' ++ us ++ Γ) fs c fk' τs params.
+Proof.
+  intros d G fs c fk ts params hok hfk us l fk' hlift;
+    inv hfk; unravel in *.
+  - destruct oe as [e |]; unravel in *.
+    + inv H0; inv H1.
+      destruct (lift_e (length us) e) as [le e'] eqn:hlifte.
+      inv hlift.
+      pose proof lift_e_type_expr
+        _ _ _ _ hok H4 _ _ _ hlifte as (ts' & hts' & Hts').
+      exists ts'. split; auto. econstructor; eauto.
+      rewrite <- H2. auto.
+    + inv H0; inv H1; inv hlift.
+      exists []; unravel; split; auto.
+      econstructor; eauto. rewrite <- H0. auto.
+  - destruct (lift_e_list (length us) cargs) as [le cargs'] eqn:hliftes.
+    inv hlift.
+    pose proof lift_e_list_type_expr
+      _ _ _ _ hok H1 _ _ _ hliftes as (ts' & hts' & Hts').
+    exists ts'. split; auto. econstructor; eauto.
+  - destruct oe as [e |]; unravel in *.
+    + inv H2; inv H3.
+      destruct (lift_e (length us) e) as [le e'] eqn:hlifte.
+      inv hlift.
+      pose proof lift_e_type_expr
+        _ _ _ _ hok H6 _ _ _ hlifte as (ts' & hts' & Hts').
+      exists ts'. split; auto. econstructor; eauto.
+      rewrite <- H4. auto.
+    + inv H2; inv H3; inv hlift.
+      exists []; unravel; split; auto.
+      econstructor; eauto. rewrite <- H2. auto.
+Qed.
+  
+Local Hint Resolve type_fun_kind_lift : core.
+Local Hint Constructors type_stmt : core.
+
+Lemma type_decl_list_unwind_vars : forall Δ Γ es τs,
+    type_decl_list Δ Γ es τs ->
+    forall fs c s sig,
+      `⧼ Δ, τs ++ Γ, fs, c ⧽ ⊢ s ⊣ sig ->
+      `⧼ Δ, Γ, fs, c ⧽ ⊢ unwind_vars es s ⊣ sig.
+Proof.
+  unfold unwind_vars.
+  intros D G es ts hes; induction hes;
+    intros fs c s sig hst; cbn in *; eauto.
+Qed.
+
+Local Hint Resolve type_decl_list_unwind_vars : core.
+Local Hint Constructors return_void_ok : core.
+
+Theorem lift_s_type_stmt : forall s Δ Γ₁ Γ₂ fs c sig,
+    Forall (t_ok Δ) Γ₁ ->
+    Forall (t_ok Δ) Γ₂ ->
+    `⧼ Δ, Γ₁ ++ Γ₂, fs, c ⧽ ⊢ s ⊣ sig -> forall τs,
+        `⧼ Δ, Γ₁ ++ τs ++ Γ₂, fs, c ⧽ ⊢ lift_s (length τs) s ⊣ sig.
+Proof.
+  intro s; induction s;
+    intros D G1 G2 fs c sig hG1 hG2 h ts; inv h; unravel; eauto.
+  - admit.
+  - admit.
+  - admit.
+  - admit.
+  - admit.
+  - destruct expr as [t | e].
+    + destruct H4 as [? hokt]; subst.
+      econstructor; eauto.
+      replace (τ :: G1 ++ ts ++ G2) with ((τ :: G1) ++ ts ++ G2) by reflexivity.
+      eauto.
+      (*
+      apply IHs.
+  - destruct c; destruct e as [e |];
+      try contradiction.
+    + inv H1; eauto.
+    + destruct return_type; try contradiction; eauto.
+      destruct (lift_e (length ts) e) as [l e'] eqn:heqlift; unravel.
+      pose proof lift_e_type_expr
+        _ _ _ _ hok H1 _ _ _ heqlift as (ts' & hts' & Hts').
+      eauto.
+    + destruct return_type; inv H1; auto.
+    + inv H1; auto.
+    + inv H1; auto.
+  - destruct (lift_trans (length ts) trns) as [le e'] eqn:hlift.
+    pose proof lift_trans_type_expr
+      _ _ _ _ hok H1 _ _ _ hlift as (ts' & hts' & Hts').
+    eauto.
+  - destruct (lift_e (length ts) lhs) as [le₁ e₁'] eqn:hlift₁.
+    destruct (lift_e (length le₁ + length ts) rhs) as [le₂ e₂'] eqn:hlift₂.
+    pose proof lift_e_type_expr
+      _ _ _ _ hok H3 _ _ _ hlift₁ as (ts₁ & hts₁ & Hts₁).
+    pose proof type_decl_list_length _ _ _ _ hts₁ as hlen₁.
+    rewrite hlen₁ in hlift₂.
+    rewrite <- app_length in hlift₂.
+    pose proof lift_e_type_expr
+      _ _ _ _ hok H5 _ _ _ hlift₂ as (ts₂ & hts₂ & Hts₂).
+    pose proof type_decl_list_length _ _ _ _ hts₂ as hlen₂.
+    rewrite <- app_assoc in hts₂, Hts₂.
+    pose proof shift_type ts₂ _ _ _ _ Hts₁ as h₂.
+    rewrite hlen₂.
+    eapply type_decl_list_unwind_vars; eauto.
+    rewrite <- app_assoc. econstructor; eauto.
+  - destruct (lift_fun_kind (length ts) call) as [lfk fk'] eqn:hliftfk.
+    pose proof type_fun_kind_lift
+      _ _ _ _ _ _ _ hok H1 _ _ _ hliftfk as (ts' & hts' & Hts').
+    admit.
+  - admit.
+  - destruct expr as [t | e].
+    + destruct H4 as [? H]; subst. econstructor; eauto.*)
+      
+      
+Admitted.
